

# DS HW2

2018-13335 Kim Kyeong Hwan

September 24, 2020

## 1

$$3 * 2^n \rightarrow n! \rightarrow 6 * n^2 \rightarrow \log_2 n \rightarrow \log_2 \log_2 n \rightarrow 2^{10}$$

## 2

- 1)c
- 2)b
- 3)b
- 4)c
- 5)a

## 3

1)

$$\begin{aligned}T(n) &= 2T(n-1) + 1 \\T(n) + 1 &= 2T(n-1) + 2 \\T(n) + 1 &= 2(T(n-1) + 1) \text{ (let } T(n) + 1 = T'(n)) \\T'(n) &= 2T'(n-1) \\T'(n) &= 2^{n-1} * T'(1) \\T(n) &= 2^n - 1\end{aligned}$$

2)

Let  $T''(n)$  is Y machine time complexity  
then  $T''(n) = T(n)/128 = t/128$   
 $T''(n+7) = t$   
Therefore We can process  $n+7$  inputs in  $t$  seconds in Y

## 4

1)

This code runs until  $s = 1 + 2 + \dots i = i * (i + 1) / 2 < n$  and it runs  $i$  times.  
Therefore time complexity is  $\Theta(\sqrt{n})$

2)

This code runs  $n$  times and  $m$  times.  
So time complexity is  $\Theta(n + m)$

3)

This code runs  $n(n + 1) / 2$  times and  $n$  times  
So time complexity is  $\Theta(n^2)$

4) Let running time  $T(n)$ , then  $T(n) = T(n - 1) + c$  ( $c$  is constant)  
 $T(n) = T(n - 2) + 2c = \dots = nc$   
So time complexity is  $\Theta(n)$

## 5

1)

Let running time  $T(n)$   
Then  $T(n) = T(n - 1) + c$  ( $c$  is constant,  $T(0) = 1$ )  
 $T(n) = T(n - 1) + c = T(n - 2) + 2c = \dots = T(0) + nc$   
Therefore  $T(n) = \Theta(n)$

2)

Let running time  $T(n)$   
Then  $T(n) = T(n/2) + c$  ( $c$  is constant,  $T(0) = 1$ )  
 $T(n) = T(n/2) + c = T(n/4) + 2c = \dots = T(1) + \log_2(n)$   
Therefore  $T(n) = \Theta(\log(n))$